simplify theta_c soundness proof with fancy tactics

Clean/Gadgets/Keccak/Keccak.lean
@@ -1,9 +1,11 @@
 import Mathlib.Tactic.Linarith.Frontend
 import Clean.Types.U64
-
+import Clean.Gadgets.Rotation64.Theorems
 namespace Clean.Gadgets.Keccak256
 
-def RoundConstants : Vector UInt64 24 := #v[
+open Gadgets.Rotation64.Theorems (rot_right64)
+
+def RoundConstants : Vector ℕ 24 := #v[
   0x0000000000000001, 0x0000000000008082,
   0x800000000000808a, 0x8000000080008000,
   0x000000000000808b, 0x0000000080000001,
@@ -15,28 +17,25 @@ def RoundConstants : Vector UInt64 24 := #v[
   0x8000000000008002, 0x8000000000000080,
   0x000000000000800a, 0x800000008000000a,
   0x8000000080008081, 0x8000000000008080,
-  0x0000000080000001, 0x8000000080008008]
+  0x0000000080000001, 0x8000000080008008
+]
 
 def bits2bytes (x : Nat) : Nat :=
   (x + 7) / 8
 
-def xor_u64 (a b : UInt64) : UInt64 := a ^^^ b
+@[reducible]
+def xor_u64 (a b : ℕ) : ℕ := a.xor b
 
-def not_u64 (a : UInt64) : UInt64 := a ^^^ 0xffffffffffffffff
+def not_u64 (a : ℕ) : ℕ := a ^^^ 0xffffffffffffffff
 
-def and_u64 (a b : UInt64) : UInt64 := a &&& b
+def and_u64 (a b : ℕ) : ℕ := a &&& b
 
-def rol_u64 (value : UInt64) (left : Nat) : UInt64:=
-  let value := value.toNat
-  let left := (64 - left) % 64
-  let low := value % (2^left)
-  let high := value / (2^left)
-  let low := low * (2^(64 - left))
-  let res := low + high
-  UInt64.ofNat res
+def rol_u64 (value : ℕ) (left : Nat) : ℕ:=
+  let right := (64 - left) % 64
+  rot_right64 value right
 
 
-def theta_c (state : Vector UInt64 25) : Vector UInt64 5 :=
+def theta_c (state : Vector ℕ 25) : Vector ℕ 5 :=
     #v[
       xor_u64 (xor_u64 (xor_u64 (xor_u64 (state.get 0) (state.get 1)) (state.get 2)) (state.get 3)) (state.get 4),
       xor_u64 (xor_u64 (xor_u64 (xor_u64 (state.get 5) (state.get 6)) (state.get 7)) (state.get 8)) (state.get 9),
@@ -45,7 +44,7 @@ def theta_c (state : Vector UInt64 25) : Vector UInt64 5 :=
       xor_u64 (xor_u64 (xor_u64 (xor_u64 (state.get 20) (state.get 21)) (state.get 22)) (state.get 23)) (state.get 24)
     ]
 
-def theta_d (c : Vector UInt64 5) : Vector UInt64 5 :=
+def theta_d (c : Vector ℕ 5) : Vector ℕ 5 :=
   #v[
     xor_u64 (c.get 4) (rol_u64 (c.get 1) 1),
     xor_u64 (c.get 0) (rol_u64 (c.get 2) 1),
@@ -55,7 +54,7 @@ def theta_d (c : Vector UInt64 5) : Vector UInt64 5 :=
   ]
 
 
-def theta_xor (state : Vector UInt64 25) (d : Vector UInt64 5) : Vector UInt64 25 :=
+def theta_xor (state : Vector ℕ 25) (d : Vector ℕ 5) : Vector ℕ 25 :=
   #v[
     xor_u64 (state.get 0) (d.get 0),
     xor_u64 (state.get 1) (d.get 0),
@@ -84,12 +83,12 @@ def theta_xor (state : Vector UInt64 25) (d : Vector UInt64 5) : Vector UInt64 2
     xor_u64 (state.get 24) (d.get 4)
   ]
 
-def theta (state : Vector UInt64 25) : Vector UInt64 25 :=
+def theta (state : Vector ℕ 25) : Vector ℕ 25 :=
   let c := theta_c state
   let d := theta_d c
   theta_xor state d
 
-def rho_phi (state : Vector UInt64 25) : Vector UInt64 25 :=
+def rho_phi (state : Vector ℕ 25) : Vector ℕ 25 :=
   #v[
     rol_u64 (state.get 0) 0,
     rol_u64 (state.get 15) 28,
@@ -118,7 +117,7 @@ def rho_phi (state : Vector UInt64 25) : Vector UInt64 25 :=
     rol_u64 (state.get 9) 2
   ]
 
-def chi (b : Vector UInt64 25) : Vector UInt64 25 :=
+def chi (b : Vector ℕ 25) : Vector ℕ 25 :=
   #v[
     xor_u64 (b.get 0) (and_u64 (not_u64 (b.get 5)) (b.get 10)),
     xor_u64 (b.get 1) (and_u64 (not_u64 (b.get 6)) (b.get 11)),
@@ -147,18 +146,18 @@ def chi (b : Vector UInt64 25) : Vector UInt64 25 :=
     xor_u64 (b.get 24) (and_u64 (not_u64 (b.get 4)) (b.get 9))
   ]
 
-def iota (state : Vector UInt64 25) (rc : UInt64) : Vector UInt64 25 :=
+def iota (state : Vector ℕ 25) (rc : ℕ) : Vector ℕ 25 :=
   state.set 0 (xor_u64 rc <| state.get 0)
 
 
-def keccak_round (state : Vector UInt64 25) (rc : UInt64) : Vector UInt64 25 :=
+def keccak_round (state : Vector ℕ 25) (rc : ℕ) : Vector ℕ 25 :=
   let theta_state := theta state
   let rho_phi_state := rho_phi theta_state
   let chi_state := chi rho_phi_state
   iota chi_state rc
 
-def keccak_f (state : Vector UInt64 25): Vector UInt64 25 :=
-  let rec keccak_f_aux (state : Vector UInt64 25) (i : ℕ) : Vector UInt64 25 :=
+def keccak_f (state : Vector ℕ 25): Vector ℕ 25 :=
+  let rec keccak_f_aux (state : Vector ℕ 25) (i : ℕ) : Vector ℕ 25 :=
     match i with
     | 0 => state
     | i + 1 =>
@@ -201,11 +200,11 @@ def state : Vector (U64 ℕ) 25 := #v[
 ]
 -- state = [[67, 168, 144, 181, 2, 173, 144, 47], [114, 52, 107, 105, 171, 22, 114, 75], [196, 118, 22, 253, 100, 162, 87, 52], [50, 65, 171, 81, 229, 6, 172, 155], [178, 167, 68, 225, 82, 73, 216, 194], [193, 5, 52, 193, 148, 168, 64, 147], [212, 142, 107, 244, 55, 237, 100, 203], [101, 34, 195, 62, 133, 216, 64, 34], [240, 214, 204, 27, 17, 231, 66, 179], [136, 37, 228, 137, 64, 208, 27, 90], [177, 229, 130, 4, 191, 7, 25, 117], [124, 168, 245, 7, 222, 138, 168, 16], [115, 130, 213, 74, 217, 123, 172, 109], [128, 149, 137, 6, 45, 133, 77, 101], [104, 90, 153, 237, 72, 44, 164, 84], [129, 177, 235, 28, 82, 30, 150, 201], [52, 55, 32, 241, 142, 211, 246, 68], [149, 124, 124, 204, 34, 220, 229, 69], [215, 168, 47, 96, 70, 5, 220, 2], [53, 224, 38, 18, 110, 66, 70, 9], [213, 122, 200, 196, 186, 122, 207, 42], [141, 103, 32, 88, 244, 160, 37, 76], [99, 242, 138, 24, 4, 30, 100, 196], [141, 253, 136, 54, 8, 21, 204, 152], [93, 161, 29, 12, 44, 252, 49, 57]]
 
-def state' := state.map (λ x => x |> U64.value_nat |> UInt64.ofNat)
+def state' := state.map (λ x => x |> U64.value_nat)
 
 def rc : U64 ℕ := ⟨235, 226, 178, 113, 2, 17, 87, 249⟩
 #eval theta state' |> rho_phi |> chi
-#eval keccak_f state' |>.map (λ x => x |> UInt64.toNat |> U64.decompose_nat_nat)
+#eval keccak_f state' |>.map (λ x => x |> U64.decompose_nat_nat)
 -- [[158, 112, 239, 65, 247, 184, 42, 29],[18, 33, 104, 153, 4, 113, 230, 164], [203, 128, 138, 52, 66, 249, 134, 137], [204, 130, 87, 203, 75, 229, 26, 49], [101, 124, 134, 181, 193, 247, 248, 194], [170, 160, 115, 17, 65, 59, 26, 242], [211, 14, 202, 60, 11, 138, 72, 44], [21, 90, 64, 58, 127, 167, 131, 94], [242, 160, 171, 170, 232, 135, 11, 166], [172, 234, 194, 74, 41, 176, 182, 229], [174, 35, 251, 95, 139, 151, 128, 196], [140, 76, 0, 166, 43, 181, 26, 214], [15, 95, 132, 163, 192, 11, 248, 213], [99, 110, 8, 73, 127, 107, 70, 240], [208, 251, 207, 18, 172, 113, 72, 220], [166, 119, 55, 190, 184, 224, 76, 193], [132, 182, 193, 105, 46, 92, 159, 3], [161, 219, 100, 118, 249, 82, 69, 168], [3, 191, 204, 13, 134, 22, 134, 93], [250, 46, 70, 133, 112, 75, 14, 27], [230, 133, 192, 229, 9, 245, 148, 47], [41, 51, 79, 61, 157, 210, 157, 201], [81, 88, 205, 113, 250, 141, 5, 116], [137, 227, 13, 73, 228, 151, 175, 151], [62, 184, 103, 254, 5, 201, 102, 121]]
 
 end Clean.Gadgets.Keccak256.Tests
