Clean/Gadgets/Rotation64/Rotation64.lean
@@ -10,7 +10,7 @@ namespace Gadgets.Rotation64
 variable {p : ℕ} [Fact p.Prime]
 variable [p_large_enough: Fact (p > 512)]
 
-open Gadgets.Rotation64.Theorems (rot_right64 rot_right8)
+open Gadgets.Rotation64.Theorems (rot_right64)
 open Gadgets.Rotation64 (byte_rotation_lookup)
 
 @[reducible]
@@ -57,7 +57,8 @@ def rot64 (offset : Fin 64) (x : Var Inputs (F p)) : Circuit (F p) (Var Outputs 
 def assumptions (input : Inputs (F p)) := input.is_normalized
 
 def spec (offset : Fin 64) (x : Inputs (F p)) (y: Outputs (F p)) :=
-  y.value = rot_right64 x.value offset.val ∧ y.is_normalized
+  y.value = rot_right64 x.value offset.val
+  ∧ y.is_normalized
 
 def circuit (off : Fin 64) : FormalCircuit (F p) Inputs Outputs where
   main := rot64 off
