Clean/Gadgets/Keccak/ThetaC.lean
@@ -3,6 +3,7 @@ import Clean.Types.U64
 import Clean.Gadgets.Addition32.Theorems
 import Clean.Gadgets.Xor.Xor64
 import Clean.Gadgets.Keccak.KeccakState
+import Clean.Gadgets.Keccak.Keccak
 
 namespace Gadgets.Keccak.ThetaC
 variable {p : ℕ} [Fact p.Prime]
@@ -10,7 +11,7 @@ variable [p_large_enough: Fact (p > 512)]
 
 open FieldUtils (mod_256 floordiv)
 open Xor (xor_u64)
-open Clean.Gadgets.Keccak256
+open Clean.Gadgets.Keccak256 (KeccakState)
 
 @[reducible] def Outputs := ProvableVector U64 5
 -- note: `reducible` is needed for type class inference, i.e. `ProvableType KeccakState`
@@ -48,20 +49,14 @@ def assumptions (state : KeccakState (F p)) : Prop :=
 
 def spec (state : KeccakState (F p)) (out: Outputs (F p)) : Prop :=
   let h_norm := out[0].is_normalized ∧ out[1].is_normalized ∧
-                out[2].is_normalized ∧ out[3].is_normalized ∧ out[4].is_normalized
+             out[2].is_normalized ∧ out[3].is_normalized ∧ out[4].is_normalized
 
-  let h_xor0 :=
-    out[0].value = (state[0].value |>.xor state[1].value |>.xor state[2].value |>.xor state[3].value |>.xor state[4].value)
-  let h_xor1 :=
-    out[1].value = (state[5].value |>.xor state[6].value |>.xor state[7].value |>.xor state[8].value |>.xor state[9].value)
-  let h_xor2 :=
-    out[2].value = (state[10].value |>.xor state[11].value |>.xor state[12].value |>.xor state[13].value |>.xor state[14].value)
-  let h_xor3 :=
-    out[3].value = (state[15].value |>.xor state[16].value |>.xor state[17].value |>.xor state[18].value |>.xor state[19].value)
-  let h_xor4 :=
-    out[4].value = (state[20].value |>.xor state[21].value |>.xor state[22].value |>.xor state[23].value |>.xor state[24].value)
+  let state_u64 := state.map (fun x => x.value)
+  let out_u64 := out.map (fun x => x.value)
 
-  h_norm ∧ (h_xor0 ∧ h_xor1 ∧ h_xor2 ∧ h_xor3 ∧ h_xor4)
+  let state' := Clean.Gadgets.Keccak256.theta_c state_u64
+
+  h_norm ∧ state' = out_u64
 
 -- #eval! theta_c (p:=p_babybear) default |>.operations.local_length
 -- #eval! theta_c (p:=p_babybear) default |>.output
@@ -83,96 +78,28 @@ theorem soundness : Soundness (F p) assumptions spec := by
   dsimp only [circuit_norm, theta_c, Xor.circuit] at h_holds
   simp only [circuit_norm, subcircuit_norm] at h_holds
   dsimp only [Xor.assumptions, Xor.spec] at h_holds
-  simp [add_assoc, and_assoc] at h_holds
+  simp [add_assoc, and_assoc, -Fin.val_zero, -Fin.val_one', -Fin.val_one, -Fin.val_two] at h_holds
 
-  -- TODO: we desperately need some abstraction here
-  have s0 : eval env (state_var[0]) = state[0] := by rw [←h_input, Vector.getElem_map]
-  have s1 : eval env (state_var[1]) = state[1] := by rw [←h_input, Vector.getElem_map]
-  have s2 : eval env (state_var[2]) = state[2] := by rw [←h_input, Vector.getElem_map]
-  have s3 : eval env (state_var[@Fin.val 25 3]) = state[3] := by rw [←h_input, Vector.getElem_map]; rfl
-  have s4 : eval env (state_var[@Fin.val 25 4]) = state[4] := by rw [←h_input, Vector.getElem_map]; rfl
-  have s5 : eval env (state_var[@Fin.val 25 5]) = state[5] := by rw [←h_input, Vector.getElem_map]; rfl
-  have s6 : eval env (state_var[@Fin.val 25 6]) = state[6] := by rw [←h_input, Vector.getElem_map]; rfl
-  have s7 : eval env (state_var[@Fin.val 25 7]) = state[7] := by rw [←h_input, Vector.getElem_map]; rfl
-  have s8 : eval env (state_var[@Fin.val 25 8]) = state[8] := by rw [←h_input, Vector.getElem_map]; rfl
-  have s9 : eval env (state_var[@Fin.val 25 9]) = state[9] := by rw [←h_input, Vector.getElem_map]; rfl
-  have s10 : eval env (state_var[@Fin.val 25 10]) = state[10] := by rw [←h_input, Vector.getElem_map]; rfl
-  have s11 : eval env (state_var[@Fin.val 25 11]) = state[11] := by rw [←h_input, Vector.getElem_map]; rfl
-  have s12 : eval env (state_var[@Fin.val 25 12]) = state[12] := by rw [←h_input, Vector.getElem_map]; rfl
-  have s13 : eval env (state_var[@Fin.val 25 13]) = state[13] := by rw [←h_input, Vector.getElem_map]; rfl
-  have s14 : eval env (state_var[@Fin.val 25 14]) = state[14] := by rw [←h_input, Vector.getElem_map]; rfl
-  have s15 : eval env (state_var[@Fin.val 25 15]) = state[15] := by rw [←h_input, Vector.getElem_map]; rfl
-  have s16 : eval env (state_var[@Fin.val 25 16]) = state[16] := by rw [←h_input, Vector.getElem_map]; rfl
-  have s17 : eval env (state_var[@Fin.val 25 17]) = state[17] := by rw [←h_input, Vector.getElem_map]; rfl
-  have s18 : eval env (state_var[@Fin.val 25 18]) = state[18] := by rw [←h_input, Vector.getElem_map]; rfl
-  have s19 : eval env (state_var[@Fin.val 25 19]) = state[19] := by rw [←h_input, Vector.getElem_map]; rfl
-  have s20 : eval env (state_var[@Fin.val 25 20]) = state[20] := by rw [←h_input, Vector.getElem_map]; rfl
-  have s21 : eval env (state_var[@Fin.val 25 21]) = state[21] := by rw [←h_input, Vector.getElem_map]; rfl
-  have s22 : eval env (state_var[@Fin.val 25 22]) = state[22] := by rw [←h_input, Vector.getElem_map]; rfl
-  have s23 : eval env (state_var[@Fin.val 25 23]) = state[23] := by rw [←h_input, Vector.getElem_map]; rfl
-  have s24 : eval env (state_var[@Fin.val 25 24]) = state[24] := by rw [←h_input, Vector.getElem_map]; rfl
-  rw [s0, s1, s2, s3, s4, s5, s6, s7, s8, s9, s10, s11, s12, s13,
-      s14, s15, s16, s17, s18, s19, s20, s21, s22, s23, s24] at h_holds
-  clear s0 s1 s2 s3 s4 s5 s6 s7 s8 s9 s10 s11 s12 s13 s14 s15 s16 s17
-    s18 s19 s20 s21 s22 s23 s24
+  have s (i : Fin 25) : eval env (state_var[i.val]) = state[i.val] := by
+    rw [←h_input, Vector.getElem_map]
 
+  simp only [s] at h_holds
   simp [circuit_norm, spec]
 
-  -- TODO ideally we would do this proof once and not 5 times!
-  -- out0 spec
-  set out0 := eval env <| var_from_offset U64 (i0 + 24)
-  obtain ⟨ h00, h01, h02, h03, h_holds ⟩ := h_holds
-  obtain ⟨ xor00, norm00 ⟩ := h00 (state_norm 0) (state_norm 1)
-  obtain ⟨ xor01, norm01 ⟩ := h01 norm00 (state_norm 2)
-  obtain ⟨ xor02, norm02 ⟩ := h02 norm01 (state_norm 3)
-  obtain ⟨ xor0, norm0 ⟩ := h03 norm02 (state_norm 4)
-  rw [xor02, xor01, xor00] at xor0
-  clear h00 h01 h02 h03 norm00 norm01 norm02 xor00 xor01 xor02
+  repeat
+    first
+    | obtain⟨ h00, h01, h02, h03, h_holds ⟩ := h_holds
+    | obtain⟨ h00, h01, h02, h03 ⟩ := h_holds
+    obtain ⟨ xor00, norm00 ⟩ := h00 (state_norm _) (state_norm _)
+    obtain ⟨ xor01, norm01 ⟩ := h01 norm00 (state_norm _)
+    obtain ⟨ xor02, norm02 ⟩ := h02 norm01 (state_norm _)
+    obtain ⟨ xor0, norm0 ⟩ := h03 norm02 (state_norm _)
+    rw [xor02, xor01, xor00] at xor0
+    clear h00 h01 h02 h03 norm00 norm01 norm02 xor00 xor01 xor02
 
-  -- out1 spec
-  set out1 := eval env <| var_from_offset U64 (i0 + 56)
-  obtain ⟨ h10, h11, h12, h13, h_holds ⟩ := h_holds
-  obtain ⟨ xor10, norm10 ⟩ := h10 (state_norm 5) (state_norm 6)
-  obtain ⟨ xor11, norm11 ⟩ := h11 norm10 (state_norm 7)
-  obtain ⟨ xor12, norm12 ⟩ := h12 norm11 (state_norm 8)
-  obtain ⟨ xor1, norm1 ⟩ := h13 norm12 (state_norm 9)
-  rw [xor12, xor11, xor10] at xor1
-  clear h10 h11 h12 h13 norm10 norm11 norm12 xor10 xor11 xor12
 
-  -- out2 spec
-  set out2 := eval env <| var_from_offset U64 (i0 + 88)
-  obtain ⟨ h20, h21, h22, h23, h_holds ⟩ := h_holds
-  obtain ⟨ xor20, norm20 ⟩ := h20 (state_norm 10) (state_norm 11)
-  obtain ⟨ xor21, norm21 ⟩ := h21 norm20 (state_norm 12)
-  obtain ⟨ xor22, norm22 ⟩ := h22 norm21 (state_norm 13)
-  obtain ⟨ xor2, norm2 ⟩ := h23 norm22 (state_norm 14)
-  rw [xor22, xor21, xor20] at xor2
-  clear h20 h21 h22 h23 norm20 norm21 norm22 xor20 xor21 xor22
-
-  -- out3 spec
-  set out3 := eval env <| var_from_offset U64 (i0 + 120)
-  obtain ⟨ h30, h31, h32, h33, h_holds ⟩ := h_holds
-  obtain ⟨ xor30, norm30 ⟩ := h30 (state_norm 15) (state_norm 16)
-  obtain ⟨ xor31, norm31 ⟩ := h31 norm30 (state_norm 17)
-  obtain ⟨ xor32, norm32 ⟩ := h32 norm31 (state_norm 18)
-  obtain ⟨ xor3, norm3 ⟩ := h33 norm32 (state_norm 19)
-  rw [xor32, xor31, xor30] at xor3
-  clear h30 h31 h32 h33 norm30 norm31 norm32 xor30 xor31 xor32
-
-  -- out4 spec
-  set out4 := eval env <| var_from_offset U64 (i0 + 152)
-  obtain ⟨ h40, h41, h42, h43 ⟩ := h_holds
-  obtain ⟨ xor40, norm40 ⟩ := h40 (state_norm 20) (state_norm 21)
-  obtain ⟨ xor41, norm41 ⟩ := h41 norm40 (state_norm 22)
-  obtain ⟨ xor42, norm42 ⟩ := h42 norm41 (state_norm 23)
-  obtain ⟨ xor4, norm4 ⟩ := h43 norm42 (state_norm 24)
-  rw [xor42, xor41, xor40] at xor4
-  clear h40 h41 h42 h43 norm40 norm41 norm42 xor40 xor41 xor42
-
-  exact ⟨
-    ⟨ norm0, norm1, norm2, norm3, norm4 ⟩,
-    ⟨ xor0, xor1, xor2, xor3, xor4 ⟩
-  ⟩
+  simp [Clean.Gadgets.Keccak256.theta_c, Clean.Gadgets.Keccak256.xor_u64, spec]
+  simp only [true_and, Fin.isValue, Fin.val_zero, Fin.val_one, Fin.val_two, *]
 
 theorem completeness : Completeness (F p) Outputs assumptions := by
   intro i0 env state_var h_env state h_input h_assumptions
